src/Language/PlutusIR/Transform/DeadCode/DSP.v
@@ -23,12 +23,15 @@ From PlutusCert Require Import
 
   SemanticEquivalence.LogicalRelation
   SemanticEquivalence.Auto
+  SemanticEquivalence.FundamentalProperty
   LetNonRec.DSP
 .
 
 Import NamedTerm.
 Import ListNotations.
 Import UniqueBinders.Term.
+
+Set Diffs "on".
 
 Lemma eval_let_subst ss r bs t v :
   Let r bs t ==> v ->
@@ -56,6 +59,8 @@ Lemma unique_typed_disjoint r bs t t' Δ Γ τ:
   Δ ,, Γ |-+ t' : τ -> (* TODO: replace with well-scoped *)
   disjoint (fv t') (bound_vars_bindings bs) .
 *)
+
+Section SubstitutionLemmas.
 
 Lemma subst_not_in_fv x t' t : ~ (In x (fv t)) -> <{ [t' / x] t }> = t.
 Admitted.
@@ -99,133 +104,165 @@ Lemma compose_subst_msubst_bindings_nonrec : forall x tx γ bs,
   <{ [ tx / x ][bnr] (/[ γ /][bnr] bs) }> = <{ /[ (x, tx) :: γ /][bnr] bs }>.
 Admitted.
 
-Lemma compat_TermBind pm_Δ pm_Γ t t' Tn b bs tb tb' x Tb Tbn :
+End SubstitutionLemmas.
+
+
+Lemma compat_TermBind pm_Δ pm_Γ t t' Tn b bs x Tb tb Tbn :
   pm_Δ |-* Tb : Kind_Base ->
   normalise Tb Tbn ->
+  (pm_Δ ,, pm_Γ |-+ tb : Tbn) ->
 
   disjoint (bvb b) (fv t') ->
-  disjoint (bvbs bs) (fv t') ->
-  Forall safe_binding bs ->
+  unique t ->
+  safe_binding b ->
 
-  forall pm_Δb pm_Γb,
+  forall pm_Δbs pm_Γbs,
     b = TermBind Strict (VarDecl x Tb) tb ->
-    pm_Δb = pm_Δ ->
-    pm_Γb = (x |-> Tbn; pm_Γ) ->
-    LR_logically_approximate pm_Δb pm_Γb (Let NonRec bs t) t' Tn ->
-    LR_logically_approximate pm_Δ  pm_Γ  tb tb' Tbn -> (* Probably not using this IH *)
-    LR_logically_approximate pm_Δ  pm_Γ  (Let NonRec (b :: bs) t) t' Tn.
+    pm_Δbs = pm_Δ ->
+    pm_Γbs = (x |-> Tbn; pm_Γ) ->
+    LR_logically_approximate pm_Δbs pm_Γbs (Let NonRec       bs  t) t' Tn ->
+    LR_logically_approximate pm_Δ   pm_Γ   (Let NonRec (b :: bs) t) t' Tn.
 Proof.
-  intros H_Tb_kind H_Tbn.
-  intros H_disjoint_b H_disjoint H_safe.
-  intros pm_Δb pm_Γb.
+  intros H_Tb_kind H_Tbn H_tb_ty.
+  intros H_disjoint_b H_unique H_safe.
+  intros pm_Δbs pm_Γbs.
   intros H_Eqb H_Δb H_Γb.
-  intros H_IH_let_bs H_IH_tb.
+  intros H_IH_let_bs.
 
   subst b.
+
+  (* Split IH in typing and evaluation *)
+  unfold LR_logically_approximate in H_IH_let_bs.
+  destruct H_IH_let_bs as [H_ty_Let [H_ty_t' H_RC]].
+
   unfold LR_logically_approximate.
   repeat split.
 
-  (* typing*)
+  (* typing *)
   1, 2: admit.
 
-    intros k ρ γ γ' Γ Δ.
-    intros H_pm_Δ_Δ H_pm_Γ_Γ.
-    intros H_Δ_ρ H_Γ_γ_γ'.
+  intros k ρ γ γ' Γ Δ.
+  intros H_pm_Δ_Δ H_pm_Γ_Γ.
+  intros H_Δ_ρ H_Γ_γ_γ'.
 
-    apply RV_to_RC.
-    autorewrite with RC.
+  apply RV_to_RC.
 
-    intros j H_lt_j_k e_f.
+  intros j H_lt_j_k e_f.
 
-    intros H_let_terminates.
-    simpl in H_let_terminates.
+  intros H_let_terminates.
 
-    rewrite msubstA_LetNonRec in H_let_terminates.
-    rewrite msubst_LetNonRec in H_let_terminates.
-    inversion H_let_terminates. subst bs0 t0 v j0.
-    clear H_let_terminates.
-    rename H3 into H_b_bs_terminate.
-    rewrite msubstA_bs_cons in H_b_bs_terminate.
-    rewrite msubst_bs_cons in H_b_bs_terminate.
-    rewrite msubstA_TermBind, msubst_TermBind in H_b_bs_terminate.
-    inversion H_b_bs_terminate. subst s x0 T t1 bs0 t0 v2.
+  rewrite msubstA_LetNonRec in H_let_terminates.
+  rewrite msubst_LetNonRec in H_let_terminates.
+  inversion H_let_terminates. subst bs0 t0 v j0.
+  clear H_let_terminates.
+  rename H3 into H_b_bs_terminate.
 
-    (* Error case*)
-    2: admit.
+  (* Push substitutions through, so we can find that
+      γρ₁(let bs = ... in t) ⇓ e_f
+  *)
+  rewrite msubstA_bs_cons, msubst_bs_cons in H_b_bs_terminate.
+  rewrite msubstA_TermBind, msubst_TermBind in H_b_bs_terminate.
+  inversion H_b_bs_terminate. subst s x0 T t1 bs0 t0 v2.
 
-    rename H9 into H_bs_terminate.
+  (* Error case*)
+  2: {
+    (** Contradiction: tb ⇓ Error, but tb is a safe binding so it should terminate *)
+    admit.
+    }
 
-    simpl in H_bs_terminate.
-    destruct
-      (* binder x should not occur as let-bound variable in bs *)
-      (existsb (eqb x) (bvbs <{ /[ γ /][bnr] (/[[ msyn1 ρ /][bnr] bs) }>)).
-      - admit. (* should be impossible by uniqueness *)
-      -
-        (* combine single substitution with multi-sibstitution *)
-        rewrite compose_subst_msubst
-              , compose_subst_msubst_bindings_nonrec in H_bs_terminate.
-        remember ((x, v1) :: γ) as γₓ.
-        remember ((x, v1) :: γ') as γ'ₓ.
+  rename H9 into H_bs_terminate.
 
-        unfold LR_logically_approximate in H_IH_let_bs.
-        repeat apply proj2 in H_IH_let_bs.
+  simpl in H_bs_terminate.
+  destruct
+    (* binder x should not occur as let-bound variable in bs *)
+    (existsb (eqb x) (bvbs <{ /[ γ /][bnr] (/[[ msyn1 ρ /][bnr] bs) }>)).
+    - admit. (* should be impossible by uniqueness *)
+    -
+      (* combine single substitution with multi-substitution *)
+      rewrite compose_subst_msubst
+            , compose_subst_msubst_bindings_nonrec in H_bs_terminate.
 
-        assert (H_γₓ_γ'ₓ : RG ρ k ((x, Tbn) :: Γ) γₓ γ'ₓ).
-        {
-         subst. eapply RG_cons.
-              all: try assumption.
-              + assert (value v1).
-                eauto using eval_to_value__eval.
-              unfold RV.
-              admit.
-              + admit.
+      (** Note about step indices
+          k  : the overall budget for let b::bs in t
+          j  : eval steps for let b::bs in t
+          j1 : eval steps for b
+          j2 : eval steps for let bs in t
+
+          j < k
+          j = j1 + 1 + j2
+      *)
+
+      (** Use fundamental property to find relates values for the
+          RHS term tb. *)
+      assert (H_LR_tb : LR_logically_approximate pm_Δ pm_Γ tb tb Tbn).
+        { auto using LR_reflexivity. }
+      destruct H_LR_tb as [_ [_ H_approx]].
+      assert
+         (H_RC_tb : RC k Tbn ρ 
+           <{ /[ γ  /] (/[[ msyn1 ρ /] tb) }>
+           <{ /[ γ' /] (/[[ msyn2 ρ /] tb) }>).
+           { eapply H_approx with (ct := Γ) (ck := Δ); auto. }
+      rewrite RV_RC in H_RC_tb.
+      specialize (H_RC_tb j1 ltac:(lia) _ H7).
+      destruct H_RC_tb as [v' [_ [_ H_RV_v1_v']]].
+
+      remember ((x, v1) :: γ) as γₓ.
+      remember ((x, v') :: γ') as γ'ₓ.
+      apply E_Let in H_bs_terminate. (* use eval instead of eval_bindings_nonrec *)
+
+      (** Construct related environments *)
+      assert (H_γₓ_γ'ₓ : RG ρ (k - j1) ((x, Tbn) :: Γ) γₓ γ'ₓ).
+      { subst γₓ γ'ₓ.
+        eapply RG_cons.
+        - eapply RV_monotone.
+          + apply H_Δ_ρ.
+          + apply H_RV_v1_v'.
+          + lia.
+        - eapply normalise_to_normal; eauto.
+        - eapply RG_monotone.
+          + apply H_Δ_ρ.
+          + apply H_Γ_γ_γ'.
+          + lia.
+      }
+
+      (* Instantiate IH with γₓ and γ'ₓ for (k - j1) steps *)
+      specialize (H_RC (k - j1) ρ γₓ γ'ₓ ((x, Tbn) :: Γ) Δ).
+      assert ( H_RC_ :
+           RC (k - j1) Tn ρ
+             <{ /[ γₓ /] (/[[ msyn1 ρ /] {Let NonRec bs t}) }>
+             <{ /[ γ'ₓ /] (/[[ msyn2 ρ /] t') }>).
+        { apply H_RC.
+          - subst. reflexivity.
+          - subst. reflexivity.
+          - apply H_Δ_ρ.
+          - apply H_γₓ_γ'ₓ.
         }
-        assert ( H_RC_ :
-             RC k Tn ρ
-               <{ /[ γₓ /] (/[[ msyn1 ρ /] {Let NonRec bs t}) }>
-               <{ /[ γ'ₓ /] (/[[ msyn2 ρ /] t') }>).
-          { apply H_IH_let_bs with   (ct := (x, Tbn) :: Γ) (ck := Δ).
-            - subst. reflexivity.
-            - subst. reflexivity.
-            - assumption.
-              (* RG ρ k ((x, Tbn) :: Γ) γₓ γ'ₓ *)
-            - assumption.
-          }
 
-        (* push substitutions through*)
-        rewrite msubstA_LetNonRec, msubst_LetNonRec in H_RC_.
+      (* push substitutions through, so we can use H_bs_terminate
+         to conclude that γ'ₓρ₂(t') ⇓ e'_f *)
+      rewrite msubstA_LetNonRec, msubst_LetNonRec in H_RC_.
+      rewrite RV_RC in H_RC_.
+      specialize (H_RC_ j2 (ltac: (lia)) _ H_bs_terminate).
+      rename H_RC_ into H_t'_terminates.
 
-        apply RC_to_RV with  (j := j2) (e_f := e_f)in H_RC_.
-        2: lia.
-        2: {
-          apply E_Let.
-          assumption.
-        }
+      destruct H_t'_terminates as [e'_f [j' [H_t'_terminates RV_e_f_e'_f]]].
+      eexists.
+      eexists.
+      split.
 
-        assert (H_RV_monotone : forall {k k' ρ e1 e2}, k' < k -> RV k Tn ρ e1 e2 -> RV k' Tn ρ e1 e2).
-        { admit. }
+      + simpl in H_disjoint_b. 
+        unfold disjoint in H_disjoint_b. 
+        apply Forall_inv in H_disjoint_b.
+        rewrite Heqγ'ₓ in H_t'_terminates.
+        rewrite msubst_not_in_fv in H_t'_terminates.
 
-        assert (H_RC_monotone : forall k k' ρ e1 e2, forall H : (k' < k), RC k Tn ρ e1 e2 -> RC k' Tn ρ e1 e2).
-        { admit. }
-
-        destruct H_RC_ as [e'_f [j' [H_t'_terminates RV_e_f_e'_f]]].
-        eexists.
-        eexists.
-        split.
-
-        + simpl in H_disjoint_b. 
-          unfold disjoint in H_disjoint_b. 
-          apply Forall_inv in H_disjoint_b.
-          rewrite Heqγ'ₓ in H_t'_terminates.
-          rewrite msubst_not_in_fv in H_t'_terminates.
-
-          apply H_t'_terminates.
-          rewrite fv_msubstA_fv.
-          assumption.
-        + eapply RV_monotone.
-          * eassumption.
-          * eassumption.
-          * lia.
+        apply H_t'_terminates.
+        rewrite fv_msubstA_fv.
+        assumption.
+      + eapply RV_monotone.
+        * eassumption.
+        * eassumption.
+        * lia.
 Admitted.
 
 
